src/Goose/Proof/Interp.v
@@ -1,0 +1,222 @@
+(* TODO: figure out a way to make this mix-in-able for anything building on Heap *)
+
+From iris.algebra Require Import auth gmap frac agree.
+Require Import Helpers.RelationTheorems.
+From iris.algebra Require Export functions csum.
+From iris.base_logic.lib Require Export invariants.
+Require Export CSL.WeakestPre CSL.Lifting CSL.Counting Count_Heap CSL.ThreadReg.
+From iris.proofmode Require Export tactics.
+
+From RecoveryRefinement.Goose Require Import Machine GoZeroValues Heap GoLayer.
+From RecoveryRefinement.Goose Require Import Machine.
+From RecoveryRefinement.Goose Require Import GoZeroValues.
+
+Set Default Proof Using "Type".
+
+Import Data.
+Import Filesys.FS.
+
+Notation heap_inG := (gen_heapG (sigT (Ptr.t)) (sigT ptrModel)).
+
+Class gooseG Σ := GooseG {
+                     go_invG : invG Σ;
+                     go_heap_inG :> heap_inG Σ;
+                     (* Maybe actually we do want a gmap version for these *)
+                     go_fs_inG :> gen_heapG string (List.list byte) Σ;
+                     go_fds_inG :> gen_heapG File (List.list byte) Σ;
+                     go_treg_inG :> tregG Σ;
+                   }.
+
+Definition heap_interp {Σ} (hM: heap_inG Σ) :=
+  (λ s, (gen_heap_ctx (SemanticsHelpers.dynMap (allocs s.(heap))) (hG := hM)))%I.
+
+Definition goose_interp {Σ} {hM: heap_inG Σ} {tr: tregG Σ} :=
+  (λ s, thread_count_interp (fst s) ∗ heap_interp hM (snd s))%I.
+
+Instance gooseG_irisG `{gooseG Σ} : irisG GoLayer.Op GoLayer.Go.l Σ :=
+  {
+    iris_invG := go_invG;
+    state_interp := goose_interp
+  }.
+
+Definition ptr_mapsto `{gooseG Σ} {T} (l: ptr T) (q: nat) (v: Datatypes.list T) : iProp Σ :=
+   mapsto (existT (Ptr.Heap T) l) q (existT (Ptr.Heap T) (Unlocked, v)).
+
+(*
+Definition path_mapsto `{baseG Σ} (p: Path) (bs: ByteString) : iProp Σ.
+Admitted.
+
+Definition fd_mapsto `{baseG Σ} (fh: Fd) (s:Path * FS.OpenMode) : iProp Σ.
+Admitted.
+*)
+
+Class GenericMapsTo `{gooseG Σ} (Addr:Type) :=
+  { ValTy : Type;
+    generic_mapsto : Addr -> nat → ValTy -> iProp Σ; }.
+
+Instance ptr_gen_mapsto `{gooseG Σ} T : GenericMapsTo (ptr T)
+  := {| generic_mapsto := ptr_mapsto; |}.
+
+Notation "l ↦{ q } v" := (generic_mapsto l q v)
+                      (at level 20) : bi_scope.
+Notation "l ↦ v" := (generic_mapsto l 0 v)
+                      (at level 20) : bi_scope.
+
+
+
+Import Reg_wp.
+Section lifting.
+Context `{gooseG Σ}.
+
+Lemma thread_reg1:
+  ∀ n σ, state_interp (n, σ)
+                      -∗ thread_count_interp n ∗ heap_interp (go_heap_inG) σ.
+Proof. auto. Qed.
+Lemma thread_reg2:
+  ∀ n σ, thread_count_interp n ∗ heap_interp (go_heap_inG) σ
+                             -∗ state_interp (n, σ).
+Proof. auto. Qed.
+
+Lemma wp_spawn {T} s E (e: proc _ T) Φ :
+  ▷ Registered
+    -∗ ▷ (Registered -∗ WP (let! _ <- e; Unregister)%proc @ s; ⊤ {{ _, True }})
+    -∗ ▷ ( Registered -∗ Φ tt)
+    -∗ WP Spawn e @ s; E {{ Φ }}.
+Proof. eapply wp_spawn; eauto using thread_reg1, thread_reg2. Qed.
+
+Lemma wp_unregister s E :
+  {{{ ▷ Registered }}} Unregister @ s; E {{{ RET tt; True }}}.
+Proof. eapply wp_unregister; eauto using thread_reg1, thread_reg2. Qed.
+
+Lemma wp_wait s E :
+  {{{ ▷ Registered }}} Wait @ s; E {{{ RET tt; AllDone }}}.
+Proof. eapply wp_wait; eauto using thread_reg1, thread_reg2. Qed.
+
+Lemma wp_ptrStore_start {T} s E (p: ptr T) off l l' v :
+  list_nth_upd l off v = Some l' →
+  {{{ ▷ p ↦ l }}}
+   Call (InjectOp.inject (PtrStore p off v SemanticsHelpers.Begin)) @ s ; E
+   {{{ RET tt; mapsto (existT (Ptr.Heap T) p) 0 (existT (Ptr.Heap T) (Locked, l)) }}}.
+Proof.
+  intros Hupd.
+  iIntros (Φ) ">Hi HΦ". rewrite /ptrStore/nonAtomicWriteOp.
+  iApply wp_lift_call_step.
+  iIntros ((n, σ)) "(?&Hσ)".
+  iDestruct (@gen_heap_valid with "Hσ Hi") as %?.
+  simpl in H0.
+  iModIntro. iSplit.
+  { destruct s; auto. iPureIntro. intros Hsnd.
+    rewrite /snd_lift in Hsnd.
+    inversion Hsnd. subst.
+    apply Eqdep.EqdepTheory.inj_pair2 in H1.
+    subst. inversion H3.
+    rewrite /readSome in H1.
+    rewrite /getAlloc in H1.
+    erewrite SemanticsHelpers.getDyn_lookup in H1; eauto.
+    congruence.
+    destruct H1 as ((?&?)&?&?&?).
+    rewrite /readSome in H1.
+    rewrite /getAlloc in H1.
+    erewrite SemanticsHelpers.getDyn_lookup in H1; eauto.
+    inversion H1. subst.
+    inversion H2.
+    rewrite /readSome in H4.
+    simpl in H4. congruence.
+    destruct H4 as (?&?&?&?).
+    rewrite //= in H4.
+  }
+  iIntros (e2 (n', σ2) Hstep) "!>".
+  inversion Hstep; subst.
+  inversion H1. subst.
+    apply Eqdep.EqdepTheory.inj_pair2 in H2.
+    subst.
+    apply Eqdep.EqdepTheory.inj_pair2 in H7.
+    subst.
+  destruct H6 as (?&?&?&?).
+  rewrite /readSome in H2. destruct x.
+  destruct H3 as (?&?&?&?).
+  rewrite /getAlloc in H2.
+    erewrite SemanticsHelpers.getDyn_lookup in H2; eauto.
+    inversion H2; subst.
+    inversion H4. subst.
+    simpl in *.
+    destruct Hstep. rewrite /goose_interp. iFrame.
+    rewrite /heap_interp//=.
+  inversion H3. subst.
+
+  unshelve (iMod (@gen_heap_update with "Hσ Hi") as "[$ Hi]").
+  iModIntro.
+  iApply "HΦ"; eauto.
+Qed.
+
+Lemma wp_ptrStore {T} s E (p: ptr T) off l l' v :
+  list_nth_upd l off v = Some l' →
+  {{{ ▷ p ↦ l }}} ptrStore p off v @ s; E {{{ RET tt; p ↦ l' }}}.
+Proof.
+  intros Hupd.
+  iIntros (Φ) ">Hi HΦ". rewrite /ptrStore/nonAtomicWriteOp.
+  wp_bind. iApply (wp_ptrStore_start with "Hi"); eauto.
+  iNext. iIntros "Hi".
+  iApply wp_lift_call_step.
+  iIntros ((n, σ)) "(?&Hσ)".
+  iDestruct (@gen_heap_valid with "Hσ Hi") as %?.
+  simpl in H0.
+  iModIntro. iSplit.
+  { destruct s; auto. iPureIntro. intros Hsnd.
+    rewrite /snd_lift in Hsnd.
+    inversion Hsnd. subst.
+    apply Eqdep.EqdepTheory.inj_pair2 in H1.
+    subst. inversion H3.
+    rewrite /readSome in H1.
+    rewrite /getAlloc in H1.
+    erewrite SemanticsHelpers.getDyn_lookup in H1; eauto.
+    congruence.
+    destruct H1 as ((?&?)&?&?&?).
+    rewrite /readSome in H1.
+    rewrite /getAlloc in H1.
+    erewrite SemanticsHelpers.getDyn_lookup in H1; eauto.
+    inversion H1. subst.
+    inversion H2.
+    rewrite /readSome in H4.
+    simpl in H4. congruence.
+    destruct H4 as (?&?&?&?).
+    rewrite //= in H4.
+    rewrite /readSome in H4. inversion H4; subst.
+    inversion H5.
+    rewrite /readSome in H6.
+    rewrite Hupd in H6. congruence.
+    destruct H6 as (?&?&?&?).
+    rewrite /readSome in H6.
+    rewrite Hupd in H6. inversion H6. subst.
+    inversion H7.
+  }
+  iIntros (e2 (n', σ2) Hstep) "!>".
+  inversion Hstep; subst.
+  inversion H1. subst.
+    apply Eqdep.EqdepTheory.inj_pair2 in H2.
+    subst.
+    apply Eqdep.EqdepTheory.inj_pair2 in H7.
+    subst.
+  destruct H6 as (?&?&?&?).
+  rewrite /readSome in H2. destruct x.
+  destruct H3 as (?&?&?&?).
+  rewrite /getAlloc in H2.
+    erewrite SemanticsHelpers.getDyn_lookup in H2; eauto.
+    inversion H2; subst.
+    inversion H4. subst.
+    simpl in *.
+    destruct Hstep. rewrite /goose_interp. iFrame.
+    rewrite /heap_interp//=.
+  inversion H3. subst.
+  destruct H5 as (?&?&?).
+  rewrite /readSome in H5. rewrite Hupd in H5. inversion H5. subst.
+  rewrite /updAllocs in H8. inversion H8. subst. simpl in *.
+  unshelve (iMod (@gen_heap_update with "Hσ Hi") as "[$ Hi]").
+  iModIntro. by iApply "HΦ".
+Qed.
+
+Lemma wp_writePtr {T} s E (p: ptr T) v' l v :
+  {{{ ▷ p ↦ (v' :: l) }}} writePtr p v @ s; E {{{ RET tt; p ↦ (v :: l) }}}.
+Proof. iIntros (Φ) ">Hi HΦ". iApply (wp_ptrStore with "Hi"); eauto. Qed.
+
+End lifting.
